formal/codegen-ptx/PtxKernelSpec.mli
@@ -1,10 +1,18 @@
 open AGpuSemantics
+open Ascii
 open PtxStmtSpec
 open String
+
+type ir_shared_decl = {shdecl_name : string; shdecl_size : int}
+
+val shdecl_name : ir_shared_decl -> string
+
+val shdecl_size : ir_shared_decl -> int
 
 type ir_kernel = {
   kern_name : string;
   kern_params : string list;
+  kern_shared : ir_shared_decl list;
   kern_body : ir_stmt;
 }
 
@@ -12,17 +20,22 @@ val kern_name : ir_kernel -> string
 
 val kern_params : ir_kernel -> string list
 
+val kern_shared : ir_kernel -> ir_shared_decl list
+
 val kern_body : ir_kernel -> ir_stmt
 
 type ptx_kernel_ast = {
   ptx_kern_name : string;
   ptx_kern_params : string list;
+  ptx_kern_shared : ir_shared_decl list;
   ptx_kern_body : ptx_stmt_ast;
 }
 
 val ptx_kern_name : ptx_kernel_ast -> string
 
 val ptx_kern_params : ptx_kernel_ast -> string list
+
+val ptx_kern_shared : ptx_kernel_ast -> ir_shared_decl list
 
 val ptx_kern_body : ptx_kernel_ast -> ptx_stmt_ast
 
@@ -31,3 +44,17 @@ val agpu_exec_ir_kernel : agpu_state -> ir_kernel -> agpu_state option
 val agpu_exec_ptx_kernel : agpu_state -> ptx_kernel_ast -> agpu_state option
 
 val emit_ast_kernel : ir_kernel -> ptx_kernel_ast
+
+val ex_empty_regs : string -> ptx_val option
+
+val ex_zero_tc : thread_const
+
+val ex_zero_mem : agpu_mem
+
+val ex_st : agpu_state
+
+val ex_k_no_shared : ir_kernel
+
+val ex_shared_decl : ir_shared_decl
+
+val ex_k_with_shared : ir_kernel
